Foundation/FirstOrder/Arithmetic/ISigma1/Prenex.lean
@@ -24,12 +24,12 @@ lemma nonempty_strictHierarchyFormulaEquivOf {φ : ArithmeticSemisentence n} (h 
 
 lemma exists_strictHierarchy_provable {φ : ArithmeticSemisentence n} (h : Hierarchy 𝚺 1 φ) :
     ∃ θ : ArithmeticSemisentence (n + 1), Hierarchy 𝚺 0 θ ∧ 𝗜𝚺₁ ⊢ ∀¹* (φ 🡘 ∃¹ θ) := by
-  obtain ⟨Φ⟩ := nonempty_strictHierarchyFormulaEquivOf h;
-  use (↑Φ.sigmaInv : ArithmeticSemisentence (n + 1));
+  obtain ⟨φ'⟩ := nonempty_strictHierarchyFormulaEquivOf h;
+  use (↑φ'.sigmaInv : ArithmeticSemisentence (n + 1));
   and_intros;
-  . exact Φ.sigmaInv.deltaZero;
-  . rw [← Φ.coe_sigmaInv];
-    exact Φ.provable;
+  . exact φ'.sigmaInv.deltaZero;
+  . rw [← φ'.coe_sigmaInv];
+    exact φ'.provable;
 
 lemma exists_strictHierarchy_provable_of_sentence {σ : ArithmeticSentence} (h : Hierarchy 𝚺 1 σ) :
     ∃ θ : ArithmeticSemisentence 1, Hierarchy 𝚺 0 θ ∧ 𝗜𝚺₁ ⊢ σ 🡘 ∃¹ θ :=
